Change API typing strategy
Previously, the OCaml API was made type-safe by parametrising the CharInstance typeclass with a type parameter for every abstract type in the spec.
This solution would not be practical if the the number of such types grew.
As such, we now rely on an hybrid approach:
- CharInstance is not parametrized anymore: the types are member of the record (hence dependent on it);
- All functions and internal data structure stay as before (minus two type parameters);
- Functions part of the API are assigned an equivalent, yet non-dependent signature in the module used from OCaml;
- Inductive datatypes part of the API do not depent on CharInstance; they are however parametrized by type parameters;
- We use 'Marker' type classes, which are eliminated during extraction, to guide Coq's typechecking.

engines/js/Conversion.ml
@@ -4,7 +4,6 @@ module Conversion (P: Engines.EngineParameters) (S: Encoding.StringLike with typ
   module E = Engines.Engine(P)
   open E
   module Pr = Printers.Printer(P)(S)
-  open Pr
 
   type ('a, 'b) pair = {
     first: 'a;
@@ -85,7 +84,7 @@ module Conversion (P: Engines.EngineParameters) (S: Encoding.StringLike with typ
     }
   |}]
 
-  let unexotic_match_result_to_result (r: unexotic_match_result Js.Nullable.t): (character, string) Extracted.ExecArrayExotic.coq_type option =
+  let unexotic_match_result_to_result (r: unexotic_match_result Js.Nullable.t): (P.string) Extracted.ExecArrayExotic.coq_type option =
     let to_mapped_option (type a b) (f: a -> b) (o: a Js.Nullable.t): b option = Option.map f (Js.Nullable.toOption o) in
     let to_mapped_list (type a b) (f: a -> b) (a: a Js.Array.t): b list = List.map f (Array.to_list a) in
     let to_mapped_tuple (type a b c d) (f: a -> c) (g: b -> d) (p: (a, b) pair): (c * d) = (f p.first, g p.second) in
@@ -104,14 +103,14 @@ module Conversion (P: Engines.EngineParameters) (S: Encoding.StringLike with typ
         })
       )
 
-  let result_to_unexotic_match_result (r: (character, string) Extracted.ExecArrayExotic.coq_type option): unexotic_match_result Js.Nullable.t =
+  let result_to_unexotic_match_result (r: (string) Extracted.ExecArrayExotic.coq_type option): unexotic_match_result Js.Nullable.t =
     let to_mapped_nullable (type a b) (f: a -> b) (o: a option): b Js.Nullable.t = Js.Nullable.fromOption (Option.map f o) in
     let to_mapped_array (type a b) (f: a -> b) (a: a list): b Js.Array.t = Array.of_list (List.map f a) in
     let to_mapped_pair (type a b c d) (f: a -> c) (g: b -> d) (p: a * b): (c, d) pair = { first = f (fst p); second = g (snd p)} in
     let to_pair = to_mapped_pair (fun x -> x) (fun x -> x) in
     (* TODO: conversion *)
     let to_string str = (S.to_string str) in
-    r |> Option.map (fun (r: (character, string) Extracted.ExecArrayExotic.coq_type) ->
+    r |> Option.map (fun (r: (string) Extracted.ExecArrayExotic.coq_type) ->
         {
           index = r.index;
           input = to_string (r.input);
@@ -123,9 +122,9 @@ module Conversion (P: Engines.EngineParameters) (S: Encoding.StringLike with typ
       )|> Js.Nullable.fromOption
 
   module MatchResult = struct
-    let ocaml_of_js (r: Js.Re.result Js.nullable): (character, string) Extracted.ExecArrayExotic.coq_type option =
+    let ocaml_of_js (r: Js.Re.result Js.nullable): (string) Extracted.ExecArrayExotic.coq_type option =
       r |> unexotify_match_result |> unexotic_match_result_to_result
-    let js_of_ocaml (r: (character, string) Extracted.ExecArrayExotic.coq_type option): Js.Re.result Js.nullable =
+    let js_of_ocaml (r: (string) Extracted.ExecArrayExotic.coq_type option): Js.Re.result Js.nullable =
       r |> result_to_unexotic_match_result |> exotify_match_result
   end
 end
