engines/js/HostEngine.ml
@@ -8,14 +8,14 @@ module HostEngine (P: Engines.EngineParameters) (S: Encoding.StringLike with typ
   module Conversion = Conversion.Conversion(P)(S)
   type regex = Js.Re.t 
 
-  let initialize (regex: (character, string) Extracted.Patterns.coq_Regex) (flags: Extracted.RegExpFlags.coq_type): regex =
+  let initialize (regex: (character, string, P.property) Extracted.Patterns.coq_Regex) (flags: Extracted.RegExpFlags.coq_type): regex =
     let regex_string = Printer.regex_to_string ~delimited:false ~strict:true regex in
     let flags_string = Printer.flags_to_string flags in
     Js.Re.fromStringWithFlags regex_string ~flags:flags_string
 
   let setLastIndex (r: regex) (at: int): unit = Js.Re.setLastIndex r at
 
-  let exec (r: regex) (str: string): (character, string) Extracted.ExecArrayExotic.coq_type option =
+  let exec (r: regex) (str: string): (P.string) Extracted.ExecArrayExotic.coq_type option =
     let js_result = Js.Re.exec ~str:(S.to_string str) r in
     Conversion.MatchResult.ocaml_of_js (Js.Nullable.fromOption js_result)
 end
