extraction/Patterns.ml
@@ -1,23 +1,23 @@
 include Extracted.Patterns
 
-let epsilon (type c s): (c, s) coq_Regex = Empty
-let null (type c s): (c, s) coq_Regex = CharacterClass (InvertedCC EmptyCR)
+let epsilon (type c s p): (c, s, p) coq_Regex = Empty
+let null (type c s p): (c, s, p) coq_Regex = CharacterClass (InvertedCC EmptyCR)
 
 (* 'Smart' constructors for regexes *)
 module Smart = struct 
-  let disjunction (type c s) (l: (c, s) coq_Regex) (r: (c, s) coq_Regex): (c, s) coq_Regex =
+  let disjunction (type c s p) (l: (c, s, p) coq_Regex) (r: (c, s, p) coq_Regex): (c, s, p) coq_Regex =
     match l, r with
     | CharacterClass (InvertedCC EmptyCR), r -> r
     | l, CharacterClass (InvertedCC EmptyCR) -> l
     | l, r -> Disjunction (l, r)
 
-  let seq (type c s) (l: (c, s) coq_Regex) (r: (c, s) coq_Regex): (c, s) coq_Regex =
+  let seq (type c s p) (l: (c, s, p) coq_Regex) (r: (c, s, p) coq_Regex): (c, s, p) coq_Regex =
     match l, r with
     | Empty, r -> r
     | l, Empty -> l
     | l, r -> Seq (l, r)
 
-  let quantified (type c s) (r: (c, s) coq_Regex)  (min: int) (max: int option) (greedy: bool): (c, s) coq_Regex =
+  let quantified (type c s p) (r: (c, s, p) coq_Regex)  (min: int) (max: int option) (greedy: bool): (c, s, p) coq_Regex =
     let quantifierPrefix: coq_QuantifierPrefix = match max with
       | None -> RepPartialRange (min)
       | Some max -> RepRange (min, max)
