mechanization/spec/Patterns.v
@@ -5,161 +5,170 @@ From Warblre Require Import List Result Typeclasses Notation Numeric Characters.
 (* The RegExp constructor applies the following grammar to the input pattern String. An error occurs if the
   grammar cannot interpret the String as an expansion of Pattern *)
 
-Module Patterns. Section main.
-  Context `{ep: CharacterInstance Γ Σ}.
+Module Patterns.
+  Section Types.
+    Local Definition String {T: Type} `{StringMarker T} := T.
+    Local Definition Character {T: Type} `{CharacterMarker T} := T.
+    Local Definition UnicodeProperty {T: Type} `{UnicodePropertyMarker T} := T.
+    Context {Character_ String_ UnicodeProperty_: Type}
+      `{CharacterMarker Character_} `{StringMarker String_} `{UnicodePropertyMarker UnicodeProperty_}.
 
-  Definition GroupName := String.
+    Definition GroupName `{StringMarker String} := String.
 
-  (** CharacterClassEscape :: *)
-  Inductive CharacterClassEscape :=
-    (* d *)
-    | esc_d
-    (* D *)
-    | esc_D
-    (* s *)
-    | esc_s
-    (* S *)
-    | esc_S
-    (* w *)
-    | esc_w
-    (* W *)
-    | esc_W
-    (* p *)
-    | UnicodeProp (p: UnicodeProperty)
-    (* P *)
-    | UnicodePropNeg (p: UnicodeProperty).
+    (** CharacterClassEscape :: *)
+    Inductive CharacterClassEscape :=
+      (* d *)
+      | esc_d
+      (* D *)
+      | esc_D
+      (* s *)
+      | esc_s
+      (* S *)
+      | esc_S
+      (* w *)
+      | esc_w
+      (* W *)
+      | esc_W
+      (* p *)
+      | UnicodeProp (p: UnicodeProperty)
+      (* P *)
+      | UnicodePropNeg (p: UnicodeProperty).
 
-  (** ControlEscape :: *)
-  Inductive ControlEscape :=
-  (* f *)
-  | esc_f
-  (* n *)
-  | esc_n
-  (* r *)
-  | esc_r
-  (* t *)
-  | esc_t
-  (* v *)
-  | esc_v.
+    (** ControlEscape :: *)
+    Inductive ControlEscape :=
+    (* f *)
+    | esc_f
+    (* n *)
+    | esc_n
+    (* r *)
+    | esc_r
+    (* t *)
+    | esc_t
+    (* v *)
+    | esc_v.
 
-  (** RegExpUnicodeEscapeSequence :: *)
-  Inductive RegExpUnicodeEscapeSequence :=
-  | Pair (lead tail: Hex4Digits)
-  | Lonely (digis: Hex4Digits)
-  | CodePoint (c: Character).
+    (** RegExpUnicodeEscapeSequence :: *)
+    Inductive RegExpUnicodeEscapeSequence :=
+    | Pair (lead tail: Hex4Digits)
+    | Lonely (digis: Hex4Digits)
+    | CodePoint (c: Character).
 
-  (** CharacterEscape :: *)
-  Inductive CharacterEscape :=
-  | ControlEsc (esc: ControlEscape)
-  (* c *)
-  | AsciiControlEsc (l: AsciiLetter)
-  (* 0 *)
-  | esc_Zero
-  (* x *)
-  | HexEscape (d1 d2: HexDigit)
-  (* u *)
-  | UnicodeEsc (seq: RegExpUnicodeEscapeSequence)
-  | IdentityEsc (chr: Character).
+    (** CharacterEscape :: *)
+    Inductive CharacterEscape :=
+    | ControlEsc (esc: ControlEscape)
+    (* c *)
+    | AsciiControlEsc (l: AsciiLetter)
+    (* 0 *)
+    | esc_Zero
+    (* x *)
+    | HexEscape (d1 d2: HexDigit)
+    (* u *)
+    | UnicodeEsc (seq: RegExpUnicodeEscapeSequence)
+    | IdentityEsc (chr: Character).
 
+    (** ClassEscape :: *)
+    Inductive ClassEscape :=
+    (* b *)
+    | esc_b
+    (* - *)
+    | esc_Dash
+    | CCharacterClassEsc (esc: CharacterClassEscape)
+    | CCharacterEsc (esc: CharacterEscape).
 
-  (** ClassEscape :: *)
-  Inductive ClassEscape :=
-  (* b *)
-  | esc_b
-  (* - *)
-  | esc_Dash
-  | CCharacterClassEsc (esc: CharacterClassEscape)
-  | CCharacterEsc (esc: CharacterEscape).
+    (** AtomEscape :: *)
+    Inductive AtomEscape :=
+    | DecimalEsc (n: positive_integer)
+    | ACharacterClassEsc (esc: CharacterClassEscape)
+    | ACharacterEsc (esc: CharacterEscape)
+    | GroupEsc (id: GroupName).
 
-  (** AtomEscape :: *)
-  Inductive AtomEscape :=
-  | DecimalEsc (n: positive_integer)
-  | ACharacterClassEsc (esc: CharacterClassEscape)
-  | ACharacterEsc (esc: CharacterEscape)
-  | GroupEsc (id: GroupName).
+    (** QuantifierPrefix :: *)
+    Inductive QuantifierPrefix :=
+    | Star
+    | Plus
+    | Question
+    | RepExact (count: non_neg_integer)
+    | RepPartialRange (min: non_neg_integer)
+    | RepRange (min: non_neg_integer) (max: non_neg_integer).
 
-  (** QuantifierPrefix :: *)
-  Inductive QuantifierPrefix :=
-  | Star
-  | Plus
-  | Question
-  | RepExact (count: non_neg_integer)
-  | RepPartialRange (min: non_neg_integer)
-  | RepRange (min: non_neg_integer) (max: non_neg_integer).
+    (** Quantifier :: *)
+    Inductive Quantifier :=
+    | Greedy (p: QuantifierPrefix)
+    | Lazy (p: QuantifierPrefix).
 
-  (** Quantifier :: *)
-  Inductive Quantifier :=
-  | Greedy (p: QuantifierPrefix)
-  | Lazy (p: QuantifierPrefix).
+    (** ClassAtom :: *)
+    (** ClassAtomNoDash :: *)
+    Inductive ClassAtom :=
+    | SourceCharacter (chr: Character)
+    | ClassEsc (esc: ClassEscape).
 
-  (** ClassAtom :: *)
-  (** ClassAtomNoDash :: *)
-  Inductive ClassAtom :=
-  | SourceCharacter (chr: Character)
-  | ClassEsc (esc: ClassEscape).
+    (** ClassRanges :: *)
+    (** NonemptyClassRanges :: *)
+    (** NonemptyClassRangesNoDash :: *)
+    Inductive ClassRanges :=
+    | EmptyCR
+    | ClassAtomCR (ca: ClassAtom) (t: ClassRanges)
+    | RangeCR (l h: ClassAtom) (t: ClassRanges).
 
-  (** ClassRanges :: *)
-  (** NonemptyClassRanges :: *)
-  (** NonemptyClassRangesNoDash :: *)
-  Inductive ClassRanges :=
-  | EmptyCR
-  | ClassAtomCR (ca: ClassAtom) (t: ClassRanges)
-  | RangeCR (l h: ClassAtom) (t: ClassRanges).
+    (** CharacterClass :: *)
+    Inductive CharClass :=
+    | NoninvertedCC (crs: ClassRanges)
+    | InvertedCC (crs: ClassRanges).
 
-  (** CharacterClass :: *)
-  Inductive CharClass :=
-  | NoninvertedCC (crs: ClassRanges)
-  | InvertedCC (crs: ClassRanges).
-
-  (** Pattern *)
-  (** Disjunction *)
-  (** Alternative :: *)
-  (** Term :: *)
-  (** Assertion :: *)
-  (** Atom :: *)
-  Inductive Regex :=
-  | Empty
-  | Char (chr: Character)
-  | Dot
-  | AtomEsc (ae: AtomEscape)
-  | CharacterClass (cc: CharClass)
-  | Disjunction (r1 r2: Regex)
-  | Quantified (r: Regex) (q: Quantifier)
-  | Seq (r1 r2: Regex)
-  | Group (name: option GroupName) (r: Regex)
-  | InputStart (*+ ^ *)
-  | InputEnd (*+ $ *)
-  | WordBoundary (*+ \b *)
-  | NotWordBoundary (*+ \B *)
-  | Lookahead (r: Regex)
-  | NegativeLookahead (r: Regex)
-  | Lookbehind (r: Regex)
-  | NegativeLookbehind (r: Regex).
+    (** Pattern *)
+    (** Disjunction *)
+    (** Alternative :: *)
+    (** Term :: *)
+    (** Assertion :: *)
+    (** Atom :: *)
+    Inductive Regex :=
+    | Empty
+    | Char (chr: Character)
+    | Dot
+    | AtomEsc (ae: AtomEscape)
+    | CharacterClass (cc: CharClass)
+    | Disjunction (r1 r2: Regex)
+    | Quantified (r: Regex) (q: Quantifier)
+    | Seq (r1 r2: Regex)
+    | Group (name: option GroupName) (r: Regex)
+    | InputStart (*+ ^ *)
+    | InputEnd (*+ $ *)
+    | WordBoundary (*+ \b *)
+    | NotWordBoundary (*+ \B *)
+    | Lookahead (r: Regex)
+    | NegativeLookahead (r: Regex)
+    | Lookbehind (r: Regex)
+    | NegativeLookbehind (r: Regex).
+  End Types.
 
   Section EqDec.
-    #[export] #[refine] Instance eqdec_CharacterClassEscape: EqDec CharacterClassEscape := {}. decide equality; solve [ apply EqDec.eq_dec ]. Defined.
-    #[export] #[refine] Instance eqdec_ControlEscape: EqDec ControlEscape := {}. decide equality. Defined.
+    Context `{ep: CharacterInstance}.
+
+    #[export] #[refine] Instance eqdec_CharacterClassEscape: EqDec CharacterClassEscape := {}. 
+    Proof. decide equality; apply EqDec.eq_dec. Defined.
+    #[export] #[refine] Instance eqdec_ControlEscape: EqDec ControlEscape := {}.
+    Proof. decide equality. Defined.
     #[export] #[refine] Instance eqdec_Hex4Digits: EqDec Hex4Digits := {}.
-      decide equality; try apply EqDec.eq_dec. Defined.
+    Proof. decide equality; apply EqDec.eq_dec. Defined.
     #[export] #[refine] Instance eqdec_RegExpUnicodeEscapeSequence: EqDec RegExpUnicodeEscapeSequence := {}.
-      decide equality; try apply EqDec.eq_dec. Defined.
+    Proof. decide equality; apply EqDec.eq_dec. Defined.
     #[export] #[refine] Instance eqdec_CharacterEscape: EqDec CharacterEscape := {}.
-      decide equality; try apply EqDec.eq_dec. Defined.
+    Proof. decide equality; apply EqDec.eq_dec. Defined.
     #[export] #[refine] Instance eqdec_CClassEscape: EqDec ClassEscape := {}.
-      decide equality; apply EqDec.eq_dec. Defined.
+    Proof. decide equality; apply EqDec.eq_dec. Defined.
     #[export] #[refine] Instance eqdec_AtomEscape: EqDec AtomEscape := {}.
-      decide equality; try first [ apply EqDec.eq_dec ]. Defined.
+    Proof. decide equality; apply EqDec.eq_dec. Defined.
     #[export] #[refine] Instance eqdec_QuantifierPrefix: EqDec QuantifierPrefix := {}.
-      decide equality; apply EqDec.eq_dec. Defined.
+    Proof. decide equality; apply EqDec.eq_dec. Defined.
     #[export] #[refine] Instance eqdec_Quantifier: EqDec Quantifier := {}.
-      decide equality; apply EqDec.eq_dec. Defined.
+    Proof. decide equality; apply EqDec.eq_dec. Defined.
     #[export] #[refine] Instance eqdec_ClassAtom: EqDec ClassAtom := {}.
-      decide equality; apply EqDec.eq_dec. Defined.
+    Proof. decide equality; apply EqDec.eq_dec. Defined.
     #[export] #[refine] Instance eqdec_ClassRanges: EqDec ClassRanges := {}.
-      decide equality; apply EqDec.eq_dec. Defined.
+    Proof. decide equality; apply EqDec.eq_dec. Defined.
     #[export] #[refine] Instance eqdec_CharClass: EqDec CharClass := {}.
-      decide equality; apply EqDec.eq_dec. Defined.
+    Proof. decide equality; apply EqDec.eq_dec. Defined.
     #[export] #[refine] Instance eqdec_Regex: EqDec Regex := {}.
-      decide equality; apply EqDec.eq_dec. Defined.
+    Proof. decide equality; apply EqDec.eq_dec. Defined.
   End EqDec.
-End main. End Patterns.
+End Patterns.
