mechanization/spec/base/Coercions.v
@@ -19,23 +19,23 @@ Module Coercions.
 
   (* Pseudo-subtyping, a.k.a. ADTs inclusion *)
   Coercion CaptureRange_or_undefined(cr: CaptureRange) := (Some cr).
-  Coercion MatchState_or_failure `{ep: CharacterInstance Γ Σ} (x: MatchState) := (Some x).
-  Coercion CharacterClassEscape_to_ClassEscape := fun `{ep: CharacterInstance Γ Σ} (cce: CharacterClassEscape) =>CCharacterClassEsc cce.
-  Coercion CharacterEscape_to_ClassEscape := fun `{ep: CharacterInstance Γ Σ} (ce: CharacterEscape) => CCharacterEsc ce.
-  Coercion ClassEscape_to_ClassAtom := fun `{ep: CharacterInstance Γ Σ} (ce: ClassEscape) => ClassEsc ce.
-  Coercion ClassAtom_to_range := fun `{ep: CharacterInstance Γ Σ} (c: ClassAtom) => ClassAtomCR c EmptyCR.
+  Coercion MatchState_or_failure `{ep: CharacterInstance} (x: MatchState) := (Some x).
+  Coercion CharacterClassEscape_to_ClassEscape := fun `{ep: CharacterInstance} (cce: CharacterClassEscape) =>CCharacterClassEsc cce.
+  Coercion CharacterEscape_to_ClassEscape := fun `{ep: CharacterInstance} (ce: CharacterEscape) => CCharacterEsc ce.
+  Coercion ClassEscape_to_ClassAtom := fun `{ep: CharacterInstance} (ce: ClassEscape) => ClassEsc ce.
+  Coercion ClassAtom_to_range := fun `{ep: CharacterInstance} (c: ClassAtom) => ClassAtomCR c EmptyCR.
 
 
   (** These ones are used to wrap things into the error monad (Result) *)
   Coercion wrap_bool := fun (F: Type) (t: bool) => @Success _ F t.
-(*   Coercion wrap_Character := fun `{ep: CharacterInstance Γ Σ} (F: Type) (c: Character) => @Success _ F c. *)
-  Coercion wrap_list_Character := fun `{ep: CharacterInstance Γ Σ} (F: Type) (c: list Character) => @Success _ F c.
+(*   Coercion wrap_Character := fun `{ep: CharacterInstance} (F: Type) (c: Character) => @Success _ F c. *)
+  Coercion wrap_list_Character := fun `{ep: CharacterInstance} (F: Type) (c: list Character) => @Success _ F c.
 
   Coercion wrap_option := fun (F T: Type) (t: option T) => @Success _ F t.
   Coercion wrap_Result := fun (F: Type) (v: non_neg_integer) => @Success _ F v.
 
-  Coercion wrap_Matcher := fun `{ep: CharacterInstance Γ Σ} (F: Type) (m: Matcher) => @Success _ F m.
-  Coercion wrap_CharSet := fun `{ep: CharacterInstance Γ Σ} (F: Type) (s: CharSet) => @Success _ F s.
+  Coercion wrap_Matcher := fun `{ep: CharacterInstance} (F: Type) (m: Matcher) => @Success _ F m.
+  Coercion wrap_CharSet := fun `{ep: CharacterInstance} (F: Type) (s: CharSet) => @Success _ F s.
 End Coercions.
 
 #[export]
